trillium/program_logic/plain_unfolding.v
@@ -1,0 +1,216 @@
+From stdpp Require Export coPset.
+From iris.algebra Require Import gmap auth agree gset coPset.
+From iris.proofmode Require Import proofmode.
+From iris.bi.lib Require Import fixpoint_mono.
+From iris.base_logic.lib Require Export own fancy_updates.
+From iris.base_logic.lib Require Import wsat.
+From iris.base_logic Require Export later_credits physical_step derived.
+From iris.prelude Require Import options.
+Import le_upd_if.
+
+Section plain_unfolding.
+
+  Local Lemma lc_incr_supply `{!lcGS Σ} n m :
+    later_credits.lc_supply n ⊢ |==> later_credits.lc_supply (n + m) ∗ £ m.
+  Proof.
+    iIntros "H". iMod lc_zero as "H'". iCombine "H H'" as "H".
+    rewrite later_credits.lc_unseal /later_credits.lc_def later_credits.lc_supply_unseal /later_credits.lc_supply_def -!own_op.
+    iApply (own_update with "[$]").
+    eapply auth_update. eapply nat_local_update; lia.
+  Qed.
+
+  Definition lc_generator_aux `{lcGS Σ} (rec : unit → iProp Σ) (_ : unit) : iProp Σ :=
+    ∀ (P : iProp Σ) n, (£ n -∗ rec () -∗ P) ==∗ P.
+  
+  Definition lc_generator `{lcGS Σ} :=
+    bi_greatest_fixpoint lc_generator_aux.
+
+  Instance lc_generator_aux_bi_mono `{lcGS Σ} :
+    BiMonoPred (lc_generator_aux).
+  Proof.
+    split.
+    - iIntros (Φ Ψ HΦne HΨne) "#H". iIntros (E1) "HE". iIntros (P E2) "HP".
+      iApply "HE". iIntros "? ?"; iApply ("HP" with "[$]"); by iApply "H".
+    - iIntros (Φ HΦne). by intros ??? ->%leibniz_equiv.
+  Qed.
+  Lemma lc_generator_unfold `{lcGS Σ} :
+    lc_generator () ≡ lc_generator_aux lc_generator ().
+  Proof. by rewrite /lc_generator greatest_fixpoint_unfold. Qed.
+
+  Lemma lc_generator_soundness_no_lc `{!lcGpreS Σ} (Q : iProp Σ) :
+    (∀ `{!lcGS Σ}, lc_generator () -∗ Q) → ⊢ |==> Q.
+  Proof.
+    iIntros (Hfupd).
+    iMod (later_credits.le_upd.lc_alloc 0) as (Hc) "[H _]".
+    iApply Hfupd. iModIntro.
+    assert (NonExpansive (λ (u : unit), ∃ n, later_credits.lc_supply n)%I).
+    { by intros ??? ->%leibniz_equiv. }
+    iApply (greatest_fixpoint_coiter _ (λ (u : unit), ∃ n, later_credits.lc_supply n)%I with "[] [$H]").
+    iIntros "!> % (%n&Hsup) %P %m HP". iMod (lc_incr_supply with "[$]") as "[H£ Hrest]".
+    iApply ("HP" with "[$] [$]").
+  Qed.
+
+  Definition fupd_to_bupd_aux `{invGS_gen hlc Σ}
+           (rec : coPset → iProp Σ) (E1 : coPset) : iProp Σ :=
+    ∀ (P : iProp Σ) E2, ((|={E1,E2}=> rec E2 -∗ P) ==∗ ◇ P).
+
+  Definition fupd_to_bupd `{invGS_gen hlc Σ} :=
+    bi_greatest_fixpoint fupd_to_bupd_aux.
+
+  Instance fupd_to_bupd_aux_bi_mono `{invGS_gen hlc Σ} :
+    BiMonoPred (fupd_to_bupd_aux).
+  Proof.
+    split.
+    - iIntros (Φ Ψ HΦne HΨne) "#H". iIntros (E1) "HE". iIntros (P E2) "HP".
+      iApply "HE"; iMod "HP"; iModIntro. by iIntros; iApply "HP"; iApply "H".
+    - iIntros (Φ HΦne). by intros ??? ->%leibniz_equiv.
+  Qed.
+
+  Lemma fupd_to_bupd_unfold `{invGS_gen hlc Σ} E :
+    fupd_to_bupd E ≡ fupd_to_bupd_aux fupd_to_bupd E.
+  Proof. by rewrite /fupd_to_bupd greatest_fixpoint_unfold. Qed.
+
+  Lemma fupd_to_bupd_except0 `{invGS_gen hlc Σ} E E' P `{!IsExcept0 P} :
+    fupd_to_bupd E -∗ (|={E, E'}=> fupd_to_bupd E' -∗ P) ==∗ P.
+  Proof.
+    iIntros "HE HP". rewrite fupd_to_bupd_unfold.
+    iApply (is_except_0 P). iApply ("HE" with "[$]").
+  Qed.
+
+  Lemma fupd_to_bupd_except0_plain `{invGS_gen hlc Σ} E E' P `{!IsExcept0 P} `{!Plain P} :
+    fupd_to_bupd E -∗ (|={E, E'}=> fupd_to_bupd E' -∗ P) -∗ P.
+  Proof.
+    iIntros "HE HP". iApply bupd_elim. iApply (fupd_to_bupd_except0 with "[$] [$]").
+  Qed.
+
+  Lemma fupd_to_bupd_soundness_no_lc `{!invGpreS Σ} (Q : iProp Σ) :
+    (∀ `{Hinv: !invGS_gen HasNoLc Σ}, lc_generator () -∗
+      fupd_to_bupd ⊤ -∗ Q) → ⊢ |==> Q.
+  Proof.
+    iIntros (Hfupd). iApply bupd_trans.
+    iApply (@lc_generator_soundness_no_lc _ invGpreS_lc).
+    iIntros (Hc) "Hgen".
+    iMod ( @wsat_alloc _ (invGpreS0.(invGpreS_wsat))) as (Hw) "[Hw HE]".
+    set (Hi := InvG HasNoLc _ Hw Hc).
+    iApply ( @Hfupd Hi with "Hgen").
+    assert (NonExpansive (λ E, wsat ∗ ownE E)%I).
+    { by intros ??? ->%leibniz_equiv. }
+    iApply (greatest_fixpoint_coiter _ (λ E, wsat ∗ ownE E)%I with "[] [$Hw $HE]").
+    iIntros "!>" (E1) "?".
+    iIntros (P E2) "HP".
+    rewrite fancy_updates.uPred_fupd_unseal /fancy_updates.uPred_fupd_def /=.
+    iMod ("HP" with "[$]") as ">(Hw & HE & HP)".
+    do 2 iModIntro; iApply "HP"; iFrame.
+  Qed.
+
+  (* TODO: Make this opaque *)
+  Definition step_count `{!tr_generation} (ns : nat) : nat :=
+    S $ f $ physical_step.tr_per_step 0 ns.
+
+  Definition physical_step_to_laters_aux `{!tr_generation} `{invGS_gen HasNoLc Σ} `{trGS Σ} (rec : nat → iProp Σ) (ns : nat) : iProp Σ :=
+    ∀ (P : iProp Σ) (E : coPset), (fupd_to_bupd E -∗ (|={E}⧗=> fupd_to_bupd E -∗ rec (S ns) -∗ ◇■ P) -∗ ▷^(step_count ns) ◇■ P).
+  
+  Definition physical_step_to_laters `{!tr_generation} `{invGS_gen HasNoLc Σ} `{trGS Σ} :=
+    bi_greatest_fixpoint physical_step_to_laters_aux.
+  
+  Instance physical_step_to_laters_aux_bi_mono `{!tr_generation} `{invGS_gen HasNoLc Σ} `{trGS Σ} :
+    BiMonoPred (physical_step_to_laters_aux).
+  Proof.
+    split.
+    - iIntros (Φ Ψ HΦne HΨne) "#H". iIntros (n) "Hn". iIntros (P E) "HE HP".
+      iApply ("Hn" with "[$]"). iApply (physical_step_wand with "[$]"). iIntros "HP ? ?".
+      iApply ("HP" with "[$]"). by iApply "H".
+    - iIntros (Φ HΦne). by intros ??? ->%leibniz_equiv.
+  Qed.
+
+  Lemma physical_step_to_laters_unfold `{!tr_generation} `{invGS_gen HasNoLc Σ} `{trGS Σ} ns :
+    physical_step_to_laters ns ≡ physical_step_to_laters_aux physical_step_to_laters ns.
+  Proof. by rewrite /physical_step_to_laters greatest_fixpoint_unfold. Qed.
+
+  Lemma physical_step_to_laters_except0_plain `{!tr_generation} `{invGS_gen HasNoLc Σ} `{trGS Σ} ns E P `{!IsExcept0 P} `{!Plain P} :
+    physical_step_to_laters ns -∗ fupd_to_bupd E -∗ (|={E}⧗=> fupd_to_bupd E -∗ physical_step_to_laters (S ns) -∗ P) -∗ ▷^(step_count ns) P.
+  Proof.
+    iIntros "Hsteps Hfupd HP".
+    iApply (bi.laterN_wand _ (◇■ P)%I).
+    { iNext. iIntros. iApply is_except_0. iApply plainly_elim. by iApply except_0_plainly_1. }
+    rewrite physical_step_to_laters_unfold. iApply ("Hsteps" with "[$]").
+    iApply (physical_step_wand with "[$]"). iIntros "HP ? ?".
+    iApply bi.except_0_intro. iApply plain. by iApply ("HP" with "[$] [$]").
+  Qed.
+
+  Lemma foo `{invGS_gen HasNoLc Σ} {E} E' n P :
+    fupd_to_bupd E -∗ (|={E, E'}=> fupd_to_bupd E' -∗ |==> ▷^n ◇ P) -∗ |==> ▷^n ◇ P.
+  Proof.
+    iIntros "HE HP".
+    destruct n as [|n]; simpl.
+    - iApply bi.except_0_idemp. iApply bupd_trans. iApply except_0_bupd.
+      iApply (fupd_to_bupd_unfold with "HE"). iMod "HP". iIntros "!> HE".
+      by iApply "HP".
+    - iApply bi.except_0_later. iApply bi.except_0_idemp. iApply bupd_trans. iApply except_0_bupd.
+      iApply (fupd_to_bupd_unfold with "HE"). iMod "HP". iIntros "!> HE".
+      iApply bi.except_0_intro.
+      by iApply "HP".
+  Qed.
+
+  Lemma bar `{invGS_gen Σ} n Q `{!Plain Q} `{!IsExcept0 Q} :
+    fupd_to_bupd ∅  -∗ (|={∅}▷=>^n fupd_to_bupd ∅ -∗ Q) -∗ (▷^n Q).
+  Proof.
+    iIntros "HFtB HP".
+    iInduction n as [|n] "IHn".
+    { simpl. 
+      iApply is_except_0.
+      iApply bupd_elim.
+      rewrite {1}fupd_to_bupd_unfold.
+      iApply "HFtB". iApply "HP". }
+    simpl.
+    iApply bi.except_0_later.
+    iApply bupd_elim.
+    rewrite {3}fupd_to_bupd_unfold.
+    iApply "HFtB".
+    iMod "HP".
+    iIntros "!> HFtB !>".
+    iApply is_except_0.
+    { by destruct n; apply _. }
+    iApply bupd_elim.
+    rewrite {4}fupd_to_bupd_unfold.
+    iApply "HFtB".
+    iMod "HP".
+    iIntros "!> HFtB".
+    iApply ("IHn" with "HFtB HP").
+  Qed.
+
+  Lemma except_0_laterN `{invGS_gen HasNoLc Σ} n (P : iProp Σ) :
+    n ≥ 1 →
+    ◇ ▷^n P ⊢ ▷^n P.
+  Proof.
+    intros ?. destruct n; [lia|].
+    simpl. apply bi.except_0_later.
+  Qed.  
+
+  
+  Lemma physical_step_to_laters_soundness_no_lc  `{!tr_generation} `{!invGpreS Σ} `{trGpreS Σ} (Q : iProp Σ) :
+    (∀ `{invGS_gen HasNoLc Σ} `{trGS Σ}, fupd_to_bupd ⊤ -∗ physical_step_to_laters 0 -∗ Q) →
+    ⊢ |==> Q.
+  Proof.
+    iIntros (Hfupd). iApply bupd_trans. iApply fupd_to_bupd_soundness_no_lc.
+    iIntros (Hinv) "Hlc Hfupd".
+    iMod (tr_supply_alloc 0) as "(%Htr & Hsup & H⧗)"; simpl.
+    iApply ( @Hfupd _ _ with "[$]").
+    assert (NonExpansive (λ n, lc_generator () ∗ tr_supply (physical_step.tr_per_step 0 n))%I).
+    { intros ????; repeat f_equiv; eauto. }
+    iApply (greatest_fixpoint_coiter _
+      (λ n, lc_generator () ∗ tr_supply (physical_step.tr_per_step 0 n))%I with "[] [Hlc Hsup]"); [|iFrame].
+    iIntros "!>" (n) "[Hlc Htr]". rewrite /physical_step_to_laters_aux.
+    iIntros (P E) "HE HP". rewrite physical_step.physical_step_unseal /physical_step_def.
+    iApply bupd_elim. iApply (foo ∅ with "HE"). iMod "HP". iIntros "!> HE".
+    iMod tr_zero as "H⧗". iMod (tr_persistent_zero) as "H⧖".
+    iApply bupd_trans. iApply (lc_generator_unfold with "Hlc"). iIntros "H£ Hlc".
+    iSpecialize ("HP" $! _ _ _ with "[$] [$] [$] [$]").
+    (* rewrite Nat.sub_0_r. fold (step_count n). iModIntro. *)
+    iApply (bar with "[$]"). iApply (step_fupdN_wand with "[$]").
+    iIntros "!> (Hsup&_&_&_&HP) HE".
+    iApply bupd_elim. iApply (foo E 0 with "HE"). iMod "HP". iIntros "!> HE !>".
+    iApply ("HP" with "[$] [$]").
+  Qed.
+
+End plain_unfolding.
